formal-proofs/theories/lib/thread_queue/thread_queue.v
@@ -175,7 +175,7 @@ Qed.
 
 End moving_pointers.
 
-From iris.algebra Require Import list gset excl.
+From iris.algebra Require Import list gset excl csum.
 
 Section proof.
 
@@ -183,13 +183,20 @@ Notation iteratorUR := (prodUR (optionUR positiveR) mnatUR).
 Notation deqIteratorUR := iteratorUR.
 Notation enqIteratorUR := iteratorUR.
 
-Inductive cellState :=
-  | cellExchanged
-  | cellCancelled
-  | cellFilled
-  | cellAbandoned.
+Inductive cellTerminalState :=
+| cellCancelled
+| cellResumed
+| cellFilled
+| cellAbandoned.
 
-Notation cellStateUR := (prodUR (optionUR (agreeR cellState))
+Notation cellProgressUR := mnatUR.
+Definition cellUninitializedO: cellProgressUR := 0%nat.
+Definition cellInitializedO: cellProgressUR := 1%nat.
+Definition cellInhabitedO: cellProgressUR := 2%nat.
+Definition cellDoneO: cellProgressUR := 3%nat.
+
+Notation cellStateUR := (prodUR (prodUR cellProgressUR
+                                        (optionUR (agreeR cellTerminalState)))
                                 (prodUR (optionUR (exclR Qp))
                                         (optionUR (exclR unitO)))).
 
@@ -223,20 +230,118 @@ Definition tq_ap (γtq γe: gname) :=
     p_cell_invariant_persistent := cell_invariant_persistent γtq;
   |}.
 
-Theorem cell_init γtq γ id ℓ:
-  cell_cancellation_handle segment_size γ id -∗ ℓ ↦ InjLV #()
-  ={∅}=∗ inv N (cell_invariant γtq γ id ℓ).
+Theorem tq_cell_init γtq γe:
+  cell_init segment_size (tq_ap γtq γe) ∅.
 Proof.
-  rewrite /cell_init /=. iIntros "HCancHandle Hℓ".
+  rewrite /cell_init /=. iIntros "!>"  (γ id ℓ) "HCancHandle Hℓ".
   iMod (inv_alloc N _ (cell_invariant γtq γ id ℓ) with "[-]") as "#HInv".
   { iModIntro. rewrite /cell_invariant. iLeft; iFrame. }
   iModIntro. iApply "HInv".
 Qed.
 
-Definition is_thread_queue γa γtq γe γd eℓ epℓ dℓ dpℓ :=
+Theorem filter_app {A} (P: A -> Prop) {H': forall x, Decision (P x)} (l1 l2: list A):
+  filter P (l1 ++ l2) = filter P l1 ++ filter P l2.
+Proof.
+  unfold filter. induction l1; rewrite /= // /filter. rewrite IHl1.
+  by destruct (decide (P a)).
+Qed.
+
+Theorem filter_List_filter_compatible {A} (P: A -> bool) (l: list A):
+  filter P l = List.filter P l.
+Proof.
+  rewrite /filter. induction l; rewrite /= //.
+  rewrite -IHl. by destruct (P a).
+Qed.
+
+Definition count_matching {A} (P: A -> Prop) {H': forall x, Decision (P x)} (l: list A): nat :=
+  length (filter P l).
+
+Hint Unfold count_matching.
+
+Theorem count_matching_app {A} (P: A -> Prop) {H': forall x, Decision (P x)} (l1 l2: list A):
+  count_matching P (l1 ++ l2) = (count_matching P l1 + count_matching P l2)%nat.
+Proof. by rewrite /count_matching filter_app app_length. Qed.
+
+Theorem count_matching_is_sum
+        {A} (P: A -> Prop) {H': forall x, Decision (P x)}:
+  forall l,
+  let to_nat x := if decide (P x) then 1%nat else 0%nat in
+  count_matching P l = foldr (fun v a => a + to_nat v)%nat O l.
+Proof.
+  rewrite /count_matching /filter. induction l; rewrite /= //.
+  destruct (decide (P a)); rewrite /= IHl /=; lia.
+Qed.
+
+Theorem count_matching_alter
+        {A} (P: A -> Prop) {H': forall x, Decision (P x)}:
+  let to_num x := if decide (P x) then 1%nat else 0%nat in
+  forall v f l i, l !! i = Some v ->
+               count_matching P (alter f i l) =
+               (count_matching P l - (to_num v) + (to_num (f v)))%nat.
+Proof.
+  rewrite /count_matching /alter /filter. induction l; rewrite /= //.
+  case; rewrite /=.
+  { intros. simplify_eq. destruct (decide (P v)); destruct (decide (P (f v))).
+    all: rewrite /=; lia. }
+  intros n Hel. rewrite /filter /=. destruct (decide (P a)); rewrite /= IHl //.
+  destruct (decide (P v)) as [pv|]; simpl. 2: lia.
+  destruct (list_filter P H' l) eqn:Z.
+  2: destruct (decide (P (f v))); simpl; lia.
+  exfalso.
+  revert n Z Hel pv. clear. induction l.
+  - intros. inversion Hel.
+  - intros. destruct n.
+    * inversion Hel. subst. simpl in *. destruct (decide (P v)); done.
+    * inversion Hel. eapply IHl; try done. simpl in *.
+      by destruct (decide (P a)).
+Qed.
+
+Inductive cellState :=
+| cellInitialized
+| cellInhabited
+| cellDone: cellTerminalState -> cellState.
+
+Definition cellStateProgress (k: option cellState): cellProgressUR :=
+  match k with
+  | None => cellUninitializedO
+  | Some cellInitialized => cellInitializedO
+  | Some cellInhabited => cellInhabitedO
+  | Some (cellDone _) => cellDoneO
+  end.
+
+(* The cell is not part of the queue any longer. *)
+Definition wasRemoved (k: option cellState): bool :=
+  match k with
+  | Some (cellDone _) => true
+  | _ => false
+  end.
+
+Definition is_thread_queue (S R: iProp) γa γtq γe γd eℓ epℓ dℓ dpℓ :=
   let ap := tq_ap γtq γe in
   (is_infinite_array segment_size ap γa ∗
-   is_iterator segment_size γa γe eℓ epℓ ∗
-   is_iterator segment_size γa γd dℓ dpℓ)%I.
+   ∃ (enqIdx deqIdx: nat),
+   iterator_points_to segment_size γa γe eℓ epℓ enqIdx ∗
+   iterator_points_to segment_size γa γd dℓ dpℓ deqIdx ∗
+   ∃ (enqFront deqFront: nat) (l: list (option cellState)),
+     ⌜deqIdx <= deqFront⌝ ∧ ⌜enqIdx <= enqFront⌝ ∧
+     ⌜deqFront <= enqFront < length l⌝ ∧
+     ([∗ list] i ↦ k ∈ take enqFront l, if wasRemoved k then True else S)%I ∗
+     ([∗ list] i ↦ k ∈ take deqFront l, if wasRemoved k then True else R)%I ∗
+     ([∗ list] i ↦ k ∈ l,
+      match k with
+      | None => True
+      | Some cellState => ∃ ℓ, array_mapsto segment_size γa i ℓ ∗
+          match cellState with
+          | cellInitialized => ℓ ↦ NONEV ∗ cell_cancellation_handle segment_size γa i
+          | cellInhabited => (∃ (th: val), ℓ ↦ InjLV th ∗ iterator_issued γe i)
+          | cellDone cd => ℓ ↦ - ∗ match cd with
+                          | cellAbandoned => (iterator_issued γd i ∨ S)
+                          | cellCancelled => True
+                          | cellResumed => (cell_cancellation_handle segment_size γa i ∨ R)
+                          | cellFilled => (iterator_issued γe i ∨ R)
+                          end
+          end
+      end)
+  )%I.
 
 End proof.
